evaluation context pain

start.v
@@ -5,6 +5,9 @@ From Coq Require Import Arith.Arith.
 From Coq Require Import Arith.EqNat. Import Nat.
 From Coq Require Import Strings.String.
 
+(* locations are strings *)
+Definition location := string.
+Definition lifetime := string.
 
 (* RF definitions *)
 Inductive lval : Type :=
@@ -25,7 +28,7 @@ Inductive term : Type :=
   (* t1 ; t2 *)
   | TSeq (t1 t2 : term)
   (* {t} *)
-  | TBlock (t : term)
+  | TBlock (t : term) (lf : lifetime)
   (* let mut x = t *)
   | TDeclaration (x : string) (t : term)
   (* w = t *)
@@ -58,19 +61,25 @@ Inductive partial_type :=
 
 
 (* state *)
+Definition store := list (location * (partial_value * lifetime)).
 
-(* locations are strings *)
-Definition location := string.
-Definition lifetime := string.
-Definition store' := list (location * (partial_value * lifetime)).
-
-Definition s_alloc (st : store') (l : location) (pv_l : partial_value * lifetime) 
-  : store' :=
+Definition s_alloc (st : store) (l : location) (pv_l : partial_value * lifetime) 
+  : store :=
   cons (l, pv_l) st.
+
+
+Fixpoint s_in (st :store) (l : location) 
+  : partial_value * lifetime :=
+  match st with
+  | nil => (PVUndefined, "global"%string)
+  | ((cl, pv_l) :: tl)%list => if (eqb cl l) then pv_l else s_in tl l
+  end.
+
 
 Compute s_alloc nil "lx"%string (PVDefined VUnit, "l"%string).
 
 (* stuff for maps from Maps.v*)
+(*
 Definition total_map (A : Type) := string -> A.
 
 Definition t_empty {A : Type} (v : A) : total_map A :=
@@ -87,6 +96,7 @@ Notation "'_' '!->' v" := (t_empty v)
 Notation "x '!->' v ';' m" := (t_update m x v)
                               (at level 100, v at next level, right associativity).
 
+*)
 
 
 (* 
@@ -95,51 +105,28 @@ Notation "x '!->' v ';' m" := (t_update m x v)
    lifetimes : string
    locations and lifetimes maybe should not be raw strings
  *)
-Definition store := total_map (partial_value * lifetime).
+(* Definition store := total_map (partial_value * lifetime). *)
 
 
-Definition example_store :=
-  ( "x" !-> (PVDefined (VInt 1),         "l_l"%string);
-    "p" !-> (PVDefined (VBorrowRef "x"), "l_m"%string);
-    "d" !-> (PVDefined (VBorrowRef "p"), "l_f"%string);
-    "t" !-> (PVDefined (VBorrowRef "d"), "l_a"%string);
-    _ !-> (PVUndefined, ""%string)
-  ).
+Definition example_store := (
+  ("x"%string, (PVDefined (VInt 1),         "l_l"%string)) ::
+  ("p"%string, (PVDefined (VBorrowRef "x"), "l_m"%string)) ::
+  ("d"%string, (PVDefined (VBorrowRef "p"), "l_f"%string)) ::
+  ("t"%string, (PVDefined (VBorrowRef "d"), "l_a"%string)) ::
+    nil
+  )%list.
 
 (* SEMANTICS *)
 
-(*
-   loc {
-     "x" |-> <   1    >_{m},
-     "p" |-> <bref "x">_{n}
-   }, x = "x"
-
-   loc {
-     "x" |-> <   1    >_{m},
-     "p" |-> <bref "x">_{n}
-   }, *p = "x"
-
-   loc {
-     "x" |-> <   1    >_{m},
-     "p" |-> <bref "x">_{n}
-     "d" |-> <bref "p">_{n}
-   }, *d = "p"
-
-   loc {
-     "x" |-> <   1    >_{m},
-     "p" |-> <bref "x">_{n}
-     "d" |-> <bref "p">_{n}
-   }, **d = "x"
-*)
 Inductive loc : store -> lval -> location -> Prop :=
   | Loc_Var : forall (st : store) (var_loc : string), 
-      ~ (fst (st var_loc)) = PVUndefined ->
+      ~ (fst (s_in st var_loc)) = PVUndefined ->
       loc st (LVar var_loc) var_loc
   | Loc_Deref : 
       forall (st : store) (l lw: location) (w : lval),
       (
-        fst (st lw) = PVDefined (VBorrowRef l) \/
-        fst (st lw) = PVDefined (VOwnRef l)
+        fst (s_in st lw) = PVDefined (VBorrowRef l) \/
+        fst (s_in st lw) = PVDefined (VOwnRef l)
       ) ->
       loc st w lw ->
       loc st (LDeref w) l.
@@ -203,7 +190,7 @@ loc_deref "x"%string. Abort. (* we are stuck because x is not a ref*)
 
 Inductive read: store -> lval -> partial_value * lifetime -> Prop :=
   | Read : forall (st : store) (w : lval) (pv_l : partial_value * lifetime) (l : location), 
-      st l = pv_l ->
+      s_in st l = pv_l ->
       loc st w l ->
       read st w pv_l.
 
@@ -239,11 +226,8 @@ Proof.
   + loc_deref "p"%string. loc_deref "d"%string.
 Qed.
 
-Definition es_empty :=
-  ( _ !-> (PVUndefined, "global"%string)).
-
 Example read_ex5 :
-  read es_empty (LVar "x"%string) (PVUndefined, "global"%string).
+  read nil (LVar "x"%string) (PVUndefined, "global"%string).
 Proof. 
   apply Read with (l := "x"%string).
   + simpl. reflexivity.
@@ -258,23 +242,23 @@ for write to succed the location l has to already be alocated in st.
 *)
 Inductive write: store -> lval -> partial_value -> store -> Prop :=
   | Write : forall (st st' : store) (pv : partial_value) (l : location) (w : lval),
-      fst (st' l) = pv ->
+      fst (s_in st' l) = pv ->
       loc st w l ->
       write st w pv st'.
 
 
 Definition es_1 :=
-  ( "x" !-> (PVDefined (VInt 0),         "lifetime_l"%string);
-    _ !-> (PVUndefined, "global"%string)
-  ).
+  ( ("x"%string, (PVDefined (VInt 0),         "lifetime_l"%string)) ::
+    nil
+  )%list.
 
 Definition es_1' :=
-  ( "x" !-> (PVDefined (VInt 1),         "lifetime_l"%string);
-    _ !-> (PVUndefined, "global"%string)
-  ).
+  ( ("x"%string, (PVDefined (VInt 1),         "lifetime_l"%string)) ::
+    nil
+  )%list.
 
 Example write_ex1 :
-  write es_empty (LVar "x"%string) (PVDefined (VInt 0)) es_1.
+  write nil (LVar "x"%string) (PVDefined (VInt 0)) es_1.
 Proof.
   apply Write with (l := "x"%string).
   + simpl. reflexivity.
@@ -293,16 +277,16 @@ Proof.
 
 Definition es_2 :=
   ( 
-  "x" !-> (PVDefined (VInt 1),         "lifetime_l"%string);
-  "p" !-> (PVDefined (VBorrowRef "x"), "lifetime_g"%string);
-  _ !-> (PVUndefined, "global"%string)
-  ).
+  ("x"%string, (PVDefined (VInt 1),         "lifetime_l"%string)) ::
+  ("p"%string, (PVDefined (VBorrowRef "x"), "lifetime_g"%string)) ::
+  nil
+  )%list.
 Definition es_3 :=
   ( 
-  "x" !-> (PVDefined (VInt 2),         "lifetime_l"%string);
-  "p" !-> (PVDefined (VBorrowRef "x"), "lifetime_g"%string);
-  _ !-> (PVUndefined, ""%string)
-  ).
+  ("x"%string, (PVDefined (VInt 2),         "lifetime_l"%string)) ::
+  ("p"%string, (PVDefined (VBorrowRef "x"), "lifetime_g"%string)) ::
+  nil
+  )%list.
 
 Example write_ex3 :
   write es_2 (LDeref (LVar "p"%string)) (PVDefined (VInt 2)) es_3.
@@ -316,11 +300,71 @@ Qed.
 (* IMPORTANT: To implement drop correctly I fear we may have to use a non function 
    version of a store *)
 
-Fixpoint drop_locations (st : store) (l : list location) : store :=
+
+Fixpoint remove_location (st : store) (l : location) : store :=
+  match st with
+  | nil => nil
+  | (hd :: tl)%list => if (eqb l (fst hd))%string 
+      then remove_location tl l 
+      else (hd :: remove_location tl l)%list
+  end.
+
+Fixpoint remove_locations (st : store) (l : list location) : store :=
   match l with
   | nil => st
-  | cons hd tl => t_update (drop_locations st tl) hd (PVUndefined, "global"%string)
+  | cons hd tl => remove_locations (remove_location st hd) tl
   end.
+
+Fixpoint collect_in_scope (st : store) (lf : lifetime) (lst : list location)
+  : list location :=
+  match st with 
+  | nil => lst
+  | ((l, (pv, clf)) :: tl)%list => if (eqb clf lf)%string
+      then collect_in_scope tl lf (l :: lst)%list
+      else collect_in_scope tl lf lst
+  end.
+
+Fixpoint collect_pvs (st : store) (lst : list location) (pvs : list partial_value) 
+  : list partial_value :=
+  match lst with 
+  | nil => pvs
+  | (l :: tl)%list => collect_pvs st tl (fst (s_in st l) :: pvs)%list
+  end.
+
+Inductive drop : store -> list partial_value -> store -> Prop :=
+  | D_nil : forall (st : store),
+      drop st nil st
+  | D_cons_other : forall (st : store) (pv : partial_value) (tl : list partial_value),
+      (forall (l : location), (pv <> PVDefined (VOwnRef l))) ->
+      drop st (cons pv tl) st
+  | D_cons_own : forall (st1 st2 st3 : store)
+      (tl : list partial_value) (l l_own : location),
+      fst (s_in st1 l_own) = (PVDefined (VOwnRef l)) ->
+      st2 = remove_location st1 l_own ->
+      drop st2 (cons (fst (s_in st1 l)) tl) st3  ->
+      drop st1 (cons (PVDefined (VOwnRef l)) tl) st2.
+
+Definition drop_ex1_st1 : store :=
+  (
+    ("lx"%string, ((PVDefined (VInt 1)),"l"%string)) ::
+    ("lp"%string, ((PVDefined (VOwnRef "lx"%string)),"m"%string)) ::
+    nil
+  )%list.
+
+Definition drop_ex1_st2 : store :=
+  (
+    ("lx"%string, ((PVDefined (VInt 1)),"l"%string)) ::
+    nil
+  )%list.
+
+Example drop_ex1 : drop drop_ex1_st1 
+  (collect_pvs drop_ex1_st1 ("lp"%string :: nil)%list nil) 
+  drop_ex1_st2.
+Proof. simpl. apply D_cons_own with (st3 := drop_ex1_st2) (l_own := "lp"%string).
++ reflexivity.
++ reflexivity.
++ simpl. apply D_cons_other. unfold not. intros l H. injection H as H1. discriminate.
+Qed.
 
 
 Reserved Notation " t '-->' t' '|' l " (at level 40).
@@ -334,8 +378,8 @@ Inductive step : lifetime -> (term * store) -> (term * store) -> Prop :=
     write st1 w PVUndefined st2 ->
     (TMove w, st1) --> (TValue v, st2) | slf
 | R_Box : forall (v : value) (n : location) (slf : lifetime) (st1 st2 : store),
-    fst (st1 n) = PVUndefined ->
-    st2 = t_update st1 n (PVDefined v, "global"%string) ->
+    fst (s_in st1 n) = PVUndefined ->
+    st2 = cons (n, (PVDefined v, "global"%string)) st1 ->
     (THeapAlloc (TValue v), st1) --> (TValue (VOwnRef n), st2) | slf
 | R_Borrow : forall (w : lval) (lw : location) (slf : lifetime) (st : store),
     loc st w lw ->
@@ -343,44 +387,129 @@ Inductive step : lifetime -> (term * store) -> (term * store) -> Prop :=
 | R_MutBorrow : forall (w : lval) (lw : location) (slf : lifetime) (st : store),
     loc st w lw ->
     (TMutBorrow w, st) --> (TValue (VOwnRef lw), st) | slf
+| R_Assign : forall (st1 st2 st3 : store) 
+    (w : lval) (v2 : value) (pv1 : partial_value * lifetime) (slf : lifetime),
+    read st1 w pv1 ->
+    drop st1 (fst pv1 :: nil)%list st2 ->
+    write st2 w (PVDefined v2) st3 ->
+    (TAssignment w (TValue v2), st1) --> (TValue VUnit, st3) | slf
 | R_Declare : forall (v : value) (lx : location) (x : string) (slf : lifetime) (st1 st2 : store),
-    st2 = t_update st1 lx (PVDefined v, slf) ->
+    st2 = cons (lx, (PVDefined v, slf)) st1 ->
     (TDeclaration x (TValue v), st1) --> (TValue VUnit, st2) | slf
+| R_Seq : forall (st1 st2 : store) (v : value) (t : term) (slf : lifetime),
+    drop st1 (PVDefined v :: nil)%list st2 ->
+    (TSeq (TValue v) t, st1) --> (t, st2) | slf
+| R_BlockA : forall (st1 st2 : store) (l_lf m_lf : lifetime) (t1 t2 : term),
+    (t1, st1) --> (t2, st2) | m_lf ->
+    (TBlock t1 m_lf, st1) --> (TBlock t2 m_lf, st2) | l_lf
+| R_BlockB : forall (st1 st2 : store) (l_lf m_lf : lifetime) (v : value),
+    drop st1 (collect_pvs st1 (collect_in_scope st1 m_lf nil) nil) st2 ->
+    (TBlock (TValue v) m_lf, st1) --> (TValue v, st2) | l_lf
+| R_Sub_HeapAlloc : forall (st1 st2 : store) (l_lf : lifetime) (t1 t2 : term),
+    (t1,st1) --> (t2,st2) | l_lf ->
+    (THeapAlloc t1, st1) --> (THeapAlloc t2, st2) | l_lf
+| R_Sub_Seq : forall (st1 st2 : store) (l_lf : lifetime) (t1 t2 t3 : term),
+    (t1,st1) --> (t2,st2) | l_lf ->
+    (TSeq t1 t2, st1) --> (t3, st2) | l_lf
 where " t '-->' t' '|' l " := (step l t t').
 
+(* figuring out R_Sub *)
+Open Scope list.
+Open Scope string.
 
+Definition r_sub1_st := ("y", (PVDefined (VInt 1), "l_lf")) :: nil.
+Example r_sub1: (THeapAlloc (TCopy (LVar "y")),r_sub1_st) --> 
+  (THeapAlloc (TValue (VInt 1)) ,r_sub1_st) | "l_lf".
+Proof.
+  apply R_Sub_HeapAlloc.
+  apply R_Copy with (lf := "l_lf").
+  + apply Read with (l := "y").
+    - reflexivity.
+    - loc_var.
+Qed.
 
-(* {1} *)
-Check Block (Value (Int 1)).
+Definition r_sub2_st  := ("y", (PVDefined (VInt 1), "l_lf")) :: nil.
+Definition r_sub2_st' := ("y", (PVDefined (VInt 2), "l_lf")) :: nil.
+Example r_sub2: 
+  (TSeq (TAssignment (LVar "y") (TValue (VInt 2))) (TValue VUnit)
+  ,r_sub2_st) 
+  --> 
+  (TSeq (TValue VUnit) (TValue VUnit) ,r_sub2_st') | "l_lf".
+Proof.
+  apply R_Sub_Seq. apply R_Assign with (st2 := r_sub2_st) (pv1 := (PVDefined (VInt 1), "l_lf")).
+  + apply Read with (l := "y").
+    - simpl. reflexivity.
+    - loc_var.
+  + simpl. apply D_cons_other. intros l. intros H. injection H as H1. discriminate.
+  + apply Write with (l := "y").
+    - simpl. reflexivity.
+    - loc_var.
+  Qed.
 
-(* 
+(* worked example 1 *)
 
-{
-  let mut x = box 0; 
-  {
-    let mut y = &mut x;
-    *y = box 1;
-  }; 
-  let mut z = x;
-} 
-*)
-Check Block (Seq
-  (* let mut x = box 0 *)
-  (Declaration "x" (HeapAlloc (Value (Int 0))))
-  (Seq
-    (Block (Seq 
-      (* let mut y = &mut x *)
-      (Declaration "y" (MutBorrow (Var "x"))) 
-      (Seq 
-      (* *y = box 1 *)
-        (Assignment (Deref (Var "y")) (HeapAlloc (Value (Int 1)))) 
-        (Value Unit)
-      )
-    ))
-    (Seq
-      (* let mut z = x *)
-      (Declaration "z" (Move (Var "x")))
-      (Value Unit)
+Definition we1_0 : (term * store) :=
+  (
+  TBlock (
+  TSeq 
+    (TDeclaration "x"%string (TValue (VInt 1)))
+    (
+    TSeq
+      (TDeclaration "y"%string (THeapAlloc (TCopy (LVar "x"%string))))
+      (TBlock (
+      TSeq 
+        (TDeclaration "z"%string (THeapAlloc (TValue (VInt 0))))
+        (
+        TSeq
+          (TAssignment (LVar "y"%string) (TBorrow (LVar "z"%string)))
+          (
+          TSeq
+            (TAssignment (LVar "y"%string) (TMove (LVar "z"%string)))
+            (
+            TSeq
+              (TMove (LDeref (LVar "y")))
+              (TValue VUnit)
+            )
+          )
+        )
+      ) "m_lf"%string)
     )
-  )
-).
+  ) "l_lf"%string
+  ,
+  nil
+  ).
+
+Definition we1_1 : (term * store) :=
+  (
+  TBlock (
+      (TBlock (
+      TSeq 
+        (TDeclaration "z"%string (THeapAlloc (TValue (VInt 0))))
+        (
+        TSeq
+          (TAssignment (LVar "y"%string) (TBorrow (LVar "z"%string)))
+          (
+          TSeq
+            (TAssignment (LVar "y"%string) (TMove (LVar "z"%string)))
+            (
+            TSeq
+              (TMove (LDeref (LVar "y")))
+              (TValue VUnit)
+            )
+          )
+        )
+      ) "m_lf"%string)
+  ) "l_lf"%string
+  ,
+  (
+  ("lx"%string, (PVDefined (VInt 1), "l_lf"%string)) ::
+  ("ly"%string, (PVDefined (VOwnRef "l1"%string), "l_lf"%string)) ::
+  ("l1"%string, (PVDefined (VInt 1), "global"%string)) ::
+  nil
+  )%list
+  ).
+
+Example we1_step_0_1 : we1_0 --> we1_1 | "l_lf"%string.
+Proof.
+  apply R_BlockA.
+
